lakefile.lean
@@ -3,9 +3,11 @@ open Lake DSL
 
 package «fos» {
   -- add package configuration options here
+  moreLinkArgs := #["-L./.lake/packages/LeanInfer/.lake/build/lib", "-lonnxruntime", "-lctranslate2"]
 }
+
+require LeanInfer from git "https://github.com/lean-dojo/LeanInfer.git" @ "v0.1.0"
 
 lean_lib «Fos» {
   -- add library configuration options here
 }
-
